Add comments on Spinlock examples

examples/spinlock/SpinLockMainIAProof.v
@@ -29,37 +29,51 @@ Module SpinLockMainIA. Section SpinLockMainIA.
   Lemma incr_simF : HSim.sim_fun open MA MI IstFull SpinLockMainName.incr.
   Proof.
     winit_simF u_a 0.
+    (* process src precondition *)
     wsteps_l. iDestruct "ASM" as "[[-> [TID [%γ_l [#I F]]]] ->]". hss.
     rename q2 into γ_v, q4 into ofs_v, q6 into blk_v, q8 into ofs_l, q10 into blk_l, q9 into tid.
+    (* main code *)
     wsteps_l. hss. wsteps_l. rewrite /SpinLockMainA.incr. wsteps_l.
     wsteps_r. hss. wsteps_r. rewrite /SpinLockMainI.incr. wsteps_r.
     unfold_iter_l. wsteps_l.
+    (* tgt yields *)
     sch_yield_r. iFrame; ss; clear nths; iIntros (nths st_s st_t) "IST TID".
     wsteps_r. sch_yield_r. iFrame; ss; clear nths st_s st_t; iIntros (nths st_s st_t) "IST TID".
+    (* tgt inline - lock acquire *)
     winline_r. wforce_r (tid, γ_l, Vptr blk_l ofs_l, existT 0 (lock_P (blk_v, ofs_v) γ_v)).
     wsteps_r. wforces_r. iFrame.
     iSplit; eauto. hss. wsteps_r.
     sch_yield_l. wforce_l false. wsteps_l.
+    (* start coinduction for lock acquisition *)
     iApply wsim_reset. iStopProof. revert nths. combine_quant st_s. combine_quant st_t.
     eapply wsim_coind.
     iIntros (g' [st_t [st_s nths]]) "[#I [F IST]] _ #CIH".
     unfold_iter_r. unfold_iter_l. wsteps_l. wsteps_r.
+    (* tgt yield *)
     sch_yield_r. iSplitL "IST"; ss; clear nths st_s st_t; iIntros (nths st_s st_t) "IST".
     wsteps_r. destruct q; cycle 1.
-    { wsteps_r. sch_yield_l. wforce_l false. wsteps_l. wby_coind "CIH".
-      hss. iFrame. eauto. }
+    { (* fail case *)
+      wsteps_r. sch_yield_l. wforce_l false. wsteps_l. wby_coind "CIH".
+      hss. iFrame. eauto.
+    }
+    (* success case *)
     wsteps_r. iDestruct "GRT" as "[[_ [TKN P]] <-]". hss. wsteps_r.
+    (* tgt yield *)
     sch_yield_r. iFrame; ss; clear nths st_s st_t; iIntros (nths st_s st_t) "IST TID".
     rewrite /lock_P; SL_red; iDestruct "P" as "[TKN [%x P]]"; SL_red; iDestruct "P" as "[PT P]".
+    (* tgt inline - mem load *)
     winline_r. wforce_r (blk_v, ofs_v, Vint x, 1%Qp). wforces_r. iSplitL "PT"; iFrame; eauto.
     wsteps_r. iDestruct "GRT" as "[[PT ->] ->]". hss. wsteps_r.
+    (* tgt yield *)
+    sch_yield_r. iFrame; ss; clear nths st_s st_t; iIntros (nths st_s st_t) "IST TID". wsteps_r.
     sch_yield_r. iFrame; ss; clear nths st_s st_t; iIntros (nths st_s st_t) "IST TID".
-    wsteps_r. sch_yield_r. iFrame; ss; clear nths st_s st_t; iIntros (nths st_s st_t) "IST TID".
+    (* tgt inline - mem store *)
     winline_r. wforce_r (blk_v, ofs_v, Vint (x + 1)). wforces_r. iSplitL "PT"; iFrame; eauto.
     wsteps_r. iDestruct "GRT" as "[[PT ->] ->]". hss. wsteps_r.
     sch_yield_r. iFrame; ss; clear nths st_s st_t; iIntros (nths st_s st_t) "IST TID".
     iCombine "P F" as "C". iMod (own_update with "C") as "[F C]".
     { apply frac_auth_update, (Z_local_update _ _ (x + 1) 1); lia. }
+    (* tgt inline - lock acquire - restore lock protected proposition *)
     winline_r. wforce_r (tid, γ_l, Vptr blk_l ofs_l, existT 0 (lock_P (blk_v, ofs_v) γ_v)).
     wforces_r.
     iSplitL "TID F PT TKN".
@@ -68,22 +82,28 @@ Module SpinLockMainIA. Section SpinLockMainIA.
       { iExists _; SL_red; iFrame. }
     }
     wsteps_r. hss. wsteps_r.
+    (* tgt yield *)
     sch_yield_r. iFrame; ss; clear nths st_s st_t; iIntros (nths st_s st_t) "IST".
     wsteps_r. iDestruct "GRT" as "[[-> TID] _]". hss. wsteps_r.
-    sch_yield_r. iFrame; ss; clear nths st_s st_t; iIntros (nths st_s st_t) "IST TID".
-    wsteps_r.
+    sch_yield_r. iFrame; ss; clear nths st_s st_t; iIntros (nths st_s st_t) "IST TID". wsteps_r.
+    (* src yield *)
     sch_yield_l. wsteps_l. wforce_l true. wsteps_l. wforces_l. iFrame; iSplit; eauto.
+    (* both terminate *)
     wsteps_l. wstep. iFrame. eauto.
   (*FAST*)Admitted.
 
   Lemma main_simF : HSim.sim_fun open MA MI IstFull SpinLockMainName.main.
   Proof.
     winit_simF u_a 0.
+    (* process src precondition *)
     wsteps_l. iDestruct "ASM" as "[[-> TID] ->]". hss.
+    (* tgt yield *)
     wsteps_r. sch_yield_r. iFrame; ss; clear nths; iIntros (nths st_s st_t) "IST TID".
+    (* tgt inline - mem alloc - counter allocation *)
     winline_r. wforce_r 1. wforces_r. iSplit; eauto.
     wsteps_r. iDestruct "GRT" as "[[%blk [-> [GRT _]]] ->]". hss. wsteps_r.
     wsteps_r. sch_yield_r. iFrame; ss; clear nths st_s st_t; iIntros (nths st_s st_t) "IST TID".
+    (* tgt inline - mem store - counter initialization *)
     winline_r. wforce_r (blk, 0%Z, Vint 0). wforces_r. iFrame; iSplit; eauto.
     wsteps_r. iDestruct "GRT" as "[[PT ->] ->]". hss. wsteps_r.
     wsteps_r. sch_yield_r. iFrame; ss; clear nths st_s st_t; iIntros (nths st_s st_t) "IST TID".
@@ -91,9 +111,11 @@ Module SpinLockMainIA. Section SpinLockMainIA.
     iApply (wsim_own_alloc (●F 0%Z ⋅ ◯F{1} 0%Z)).
     { eapply frac_auth_valid; ss. }
     iIntros "[%γ [B W]]".
+    (* tgt inline - newlock *)
     winline_r. wforce_r (0, existT 0 (lock_P (blk, 0%Z) γ)). wforces_r. iSplitL "TID B PT"; eauto.
     { SL_red; iSplit; eauto. iFrame. iExists _; SL_red; iFrame. }
     wsteps_r. hss. wsteps_r.
+    (* src/tgt yields *)
     sch_yield_r. iFrame; ss; clear nths st_s st_t; iIntros (nths st_s st_t) "IST".
     wsteps_r. iDestruct "GRT" as "[[TID [%val [%γ_l [-> #I]]]] %EQ]". hss. wsteps_r.
     sch_yield_r. iFrame; ss; clear nths st_s st_t; iIntros (nths st_s st_t) "IST TID".
@@ -101,6 +123,7 @@ Module SpinLockMainIA. Section SpinLockMainIA.
     sch_yield_l. wsteps_l. wforce_l (Vptr b_l o_l, Vptr blk 0). wsteps_l. sch_yield_l.
     (* create preconditions of incr *)
     iDestruct "W" as "[W1 W2]".
+    (* spawn thread 1 - incr *)
     wsteps_l. sch_spawn.
     { apply MainInSpc; ss. }
     { eapply (incr_spawnable). }
@@ -109,8 +132,10 @@ Module SpinLockMainIA. Section SpinLockMainIA.
     { iSplit; eauto. }
     iIntros (tid nths st_s st_t) "IST TID TKN".
     wsteps_l. wsteps_r.
+    (* src/tgt yields *)
     sch_yield_r. iFrame; ss; clear nths st_s st_t; iIntros (nths st_s st_t) "IST TID".
     sch_yield_l. wsteps_l.
+    (* spawn thread 2 - incr *)
     sch_spawn.
     { apply MainInSpc; ss. }
     { eapply (incr_spawnable u_a). }
@@ -119,51 +144,65 @@ Module SpinLockMainIA. Section SpinLockMainIA.
     { iSplit; eauto. }
     iIntros (tid2 nths st_s st_t) "IST TID TKN2".
     wsteps_l. wsteps_r.
+    (* src/tgt yields *)
     sch_yield_r. iFrame; ss; clear nths st_s st_t; iIntros (nths st_s st_t) "IST TID".
     sch_yield_l. wsteps_l.
+    (* join thread 1 - incr *)
     sch_join; iFrame.
     clear nths st_s st_t; iIntros (nths st_s st_t vret ret) "IST TID W1 /=".
     wsteps_r. sch_yield_r. iFrame; ss; clear nths st_s st_t; iIntros (nths st_s st_t) "IST TID".
     sch_yield_l. wsteps_l.
+    (* join thread 2 - incr *)
     sch_join; iFrame.
     clear nths st_s st_t; iIntros (nths st_s st_t vret2 ret2) "IST TID W2 /=".
     wsteps_l. wsteps_r.
     unfold_iter_l. wsteps_l.
     sch_yield_r. iFrame; ss; clear nths st_s st_t; iIntros (nths st_s st_t) "IST TID".
     sch_yield_l. wforce_l false. wsteps_l.
+    (* tgt inline - lock acquire *)
     winline_r. wforce_r (0, γ_l, Vptr b_l o_l, existT 0 (lock_P (blk, 0%Z) γ)). wforces_r. iFrame.
     iSplit; eauto.
     wsteps_r. hss. wsteps_r.
-    (* lock acquire coinduction *)
+    (* start coinduction for lock acquisition *)
     iApply wsim_reset. iStopProof. revert nths. combine_quant st_s. combine_quant st_t.
     eapply wsim_coind.
     iIntros (g' [st_t [st_s nths]]) "[#I [W1 [W2 IST]]] _ #CIH /=".
     unfold_iter_r. unfold_iter_l. wsteps_r.
+    (* tgt yield *)
     sch_yield_r. iSplitL "IST"; ss; clear nths st_s st_t; iIntros (nths st_s st_t) "IST".
     wsteps_r. destruct q; cycle 1.
-    { wsteps_r. sch_yield_l. wforce_l false. wsteps_l. wby_coind "CIH".
-      hss. iFrame. eauto. }
+    { (* fail case *)
+      wsteps_r. sch_yield_l. wforce_l false. wsteps_l. wby_coind "CIH".
+      hss. iFrame. eauto.
+    }
+    (* success case *)
     wsteps_r. iDestruct "GRT" as "[[-> [TID [TKN P]]] _]". hss. wsteps_r.
     SL_red. iCombine "W1 W2" as "W". iDestruct "P" as "[%x P]"; SL_red; iDestruct "P" as "[PT B]".
     iCombine "B W" gives %WF%frac_auth_agree. inv WF.
     sch_yield_r. iFrame; ss; clear nths st_s st_t; iIntros (nths st_s st_t) "IST TID".
+    (* tgt inline - mem load *)
     winline_r. wforce_r (blk, 0%Z, Vint 2%Z, 1%Qp). wforces_r. iSplitL "PT"; eauto.
     wsteps_r. iDestruct "GRT" as "[[PT ->] ->]". hss. wsteps_r.
+    (* tgt yield *)
     sch_yield_r. iFrame; ss; clear nths st_s st_t; iIntros (nths st_s st_t) "IST TID". wsteps_r.
     sch_yield_r. iFrame; ss; clear nths st_s st_t; iIntros (nths st_s st_t) "IST TID".
+    (* tgt inline - lock release *)
     winline_r. wforce_r (0, γ_l, Vptr b_l o_l, existT 0 (lock_P (blk, 0%Z) γ)). wforces_r.
     iSplitL "TKN TID B PT".
     { SL_red. iSplit; eauto. iFrame. iSplit; eauto. iSplit; eauto. iExists _; SL_red; iFrame. }
     wsteps_r. hss. wsteps_r.
+    (* tgt yield *)
     sch_yield_r. iFrame; ss; clear nths st_s st_t; iIntros (nths st_s st_t) "IST".
     wsteps_r. iDestruct "GRT" as "[[-> TID] _]". hss. wsteps_r.
     sch_yield_r. iFrame; ss; clear nths st_s st_t; iIntros (nths st_s st_t) "IST TID".
     sch_yield_l. wforce_l true. wsteps_l.
+    (* both output - counter value *)
     sch_yield_l. wstep.
     wsteps_l. wsteps_r.
     sch_yield_r. iFrame; ss; clear nths st_s st_t; iIntros (nths st_s st_t) "IST TID". wsteps_r.
-    sch_yield_l. wsteps_l. wforces_l. iSplit; eauto. wsteps_l. wstep.
-    iSplit; eauto.
+    sch_yield_l. wsteps_l. wforces_l. iSplit; eauto. wsteps_l.
+    (* terminate both *)
+    wstep. iSplit; eauto.
   (*FAST*)Admitted.
 
   Lemma sim : HSim.t open MA MI emp%I IstFull.
@@ -175,11 +214,11 @@ Module SpinLockMainIA. Section SpinLockMainIA.
   Qed.
 End SpinLockMainIA.
 
-Section wctxr.
+Section ctxr.
   Context `{!invG α Σ Γ, !subG Γ Σ, !sinvG Σ Γ α β τ}.
   Context `{!SchAGΣ Σ, !SchAGΓ Γ, !memGΓ Γ, !SpinLockMainAGΓ Γ, !SpinLockAGΓ Γ}.
 
-  Definition wctxr (u : univ_id) (spc_s spc_user_s spc_mem : string → option fspec)
+  Definition ctxr (u : univ_id) (spc_s spc_user_s spc_mem : string → option fspec)
       (SchInSpc : spc_incl (SchAS.spc u spc_user_s) spc_s)
       (MainInSpc : spc_incl (SpinLockMainAS.spc u) spc_user_s)
       (MemInSpc : spc_incl MemA.spc spc_s) :
@@ -187,4 +226,4 @@ Section wctxr.
       ((SpinLockMainA.t u spc_s) ★ (MemA.t u spc_mem ★ (SpinLockA.t u spc_s)), emp%I)
       ((SpinLockMainI.t)         ★ (MemA.t u spc_mem ★ (SpinLockA.t u spc_s)), emp%I).
   Proof. eapply main_adequacy, sim; eauto. Qed.
-End wctxr. End SpinLockMainIA.
+End ctxr. End SpinLockMainIA.
