examples/spinlock/SpinLockIAProof.v
@@ -1,8 +1,8 @@
 Require Import CRIS.
 
 Require Import ImpPrelude.
-Require Import SpinLockHeader SpinLockI SpinLockA SchA MemA wsim_tactics SchTactics.
-Require Import SchHeader.
+Require Import SpinLockHeader SpinLockI SpinLockA MemA wsim_tactics.
+Require Import SchHeader SchA SchTactics.
 
 Module SpinLockIA. Section SpinLockIA.
   Import SpinLockAS.
@@ -26,16 +26,22 @@ Module SpinLockIA. Section SpinLockIA.
   Lemma newlock_simF : HSim.sim_fun open MA MI IstFull SpinLockName.newlock.
   Proof.
     winit_simF u_a 0.
+    (* preprocess initial conditions *)
     wsteps_l. rename q1 into tid. destruct q2 as [n P]; s. iDestruct "ASM" as "[[TID P] ->]". hss.
+    (* tgt yield *)
     wsteps_r. sch_yield_r. iFrame. clear nths; iIntros (nths st_s st_t) "IST TID".
+    (* tgt inline - mem alloc *)
     winline_r. wforce_r 1. wforces_r. iSplit; eauto.
     wsteps_r. iDestruct "GRT" as "[[%blk [-> [PT _]]] ->]". hss. wsteps_r.
+    (* tgt yield *)
     sch_yield_r. iFrame. clear nths st_s st_t; iIntros (nths st_s st_t) "IST TID".
+    (* tgt inline - mem store *)
     winline_r. wforce_r (blk, 0%Z, Vint 0). wsteps_r. wforces_r. iSplitL "PT"; eauto.
     wsteps_r. iDestruct "GRT" as "[[PT ->] ->]". hss. wsteps_r.
+    (* src/tgt yield *)
     sch_yield_r. iFrame. clear nths st_s st_t; iIntros (nths st_s st_t) "IST TID".
     sch_yield_l. wforce_l (Vptr blk 0). wsteps_l. wforce_l. wsteps_l.
-
+    (* prove source postcondition *)
     (* alloc invariant *)
     iApply (wsim_own_alloc (Excl ())); ss. iIntros "[%γ TKN]".
     iMod (inv_alloc (SpinLockAS.lock_inv blk 0 P γ) u_a _ _ N_SpinLockA with "[P PT TKN]") as "#I"; eauto.
@@ -48,43 +54,43 @@ Module SpinLockIA. Section SpinLockIA.
   Lemma acquire_simF : HSim.sim_fun open MA MI IstFull SpinLockName.acquire.
   Proof.
     winit_simF u_a 0.
+    (* process src precondition *)
     wsteps_l. iDestruct "ASM" as "[[% [TID #LOCK]] %]". hss.
-    iDestruct "LOCK" as (? ?) "[% LOCK]".
-    wsteps_r. iApply wsim_reset.
+    iDestruct "LOCK" as (? ?) "[% LOCK]". wsteps_r.
+    (* start coinduction for lock acquire/failure *)
+    iApply wsim_reset.
     iStopProof.
-    clear NODD NODS.
-    (* revert NODUPFS. combine_quant NODUPFT. *)
-    (* combine_quant nths. *)
-    revert nths.
-    (* combine_quant NODD. combine_quant NODS. *)
-    combine_quant st_src. combine_quant st_tgt.
+    clear NODD NODS. revert nths. combine_quant st_src. combine_quant st_tgt.
     eapply wsim_coind. ii.
     destruct a as [st_tgt [st_src nths]]. ss.
     iIntros "[#LOCK [IST TID]] _ #CIH".
     unfold_iter_l. wsteps_l.
     unfold_iter_r. wsteps_r.
+    (* tgt yield *)
     sch_yield_r. iFrame. clear nths; iIntros (nths st_s st_t) "IST TID".
-    iInv "LOCK" as "I" "Hcl".
-    SL_red.
+    (* open invariant *)
+    iInv "LOCK" as "I" "Hcl". SL_red.
     iDestruct "I" as "[FAIL|SUCC]".
     { (* fail case *)
+      (* tgt inline - mem cas *)
       winline_r. wforces_r. 
       instantiate (1:= existT _ _). hss. instantiate (2:= 1). ss.
       instantiate (1:= (_, _, _, _, _)). hss. 
-      iSplitL "FAIL". iFrame. et. 
+      iSplitL "FAIL". iFrame. et.
       wsteps_r.
       iDestruct "GRT" as "[[POINTS_TO %] %]".
       hss. wsteps_r.
       iMod ("Hcl" with "[POINTS_TO]") as "_". iFrame.
-      sch_yield_r. iFrame. clear nths; iIntros (nths0 st_s0 st_t0) "IST TID".
-      wsteps_r.
-      sch_yield_r. iFrame. clear nths0; iIntros (nths st_s1 st_t1) "IST TID".
-      wsteps_r.
+      (* tgt yields *)
+      sch_yield_r. iFrame. clear nths; iIntros (nths0 st_s0 st_t0) "IST TID". wsteps_r.
+      sch_yield_r. iFrame. clear nths0; iIntros (nths st_s1 st_t1) "IST TID". wsteps_r.
+      (* src yield - choose false for looping again *)
       sch_yield_l. wforce_l false. wsteps_l.
       wby_coind "CIH".
       iFrame. done.
     }
     { (* success case *)
+      (* tgt inline - mem cas *)
       iDestruct "SUCC" as "[POINTS_TO [Q TKN]]".
       winline_r. wforces_r.
       instantiate (1:= existT _ _). ss. instantiate (2:= 0). ss.  
@@ -93,42 +99,49 @@ Module SpinLockIA. Section SpinLockIA.
       iDestruct "GRT" as "[[POINTS_TO ->] ->]". hss.
       wsteps_r.
       iMod ("Hcl" with "[POINTS_TO]") as "_". iFrame.
-      sch_yield_r. iFrame. clear nths; iIntros (nths0 st_s0 st_t0) "IST TID".
-      wsteps_r.
-      sch_yield_r. iFrame. clear nths0; iIntros (nths st_s1 st_t1) "IST TID".
-      wsteps_r.
+      (* tgt yields *)
+      sch_yield_r. iFrame. clear nths; iIntros (nths0 st_s0 st_t0) "IST TID". wsteps_r.
+      sch_yield_r. iFrame. clear nths0; iIntros (nths st_s1 st_t1) "IST TID". wsteps_r.
       sch_yield_r. iFrame. clear nths; iIntros (nths0 st_s2 st_t2) "IST TID".
+      (* src yield *)
       sch_yield_l. wforce_l true. wsteps_l. wforces_l. iSplitL "Q TKN TID"; SL_red; et. iFrame. et.
-      wstep.
-      et.
+      (* both terminate *)
+      wstep; eauto.
     }
   (*FAST*)Admitted.
 
   Lemma release_simF : HSim.sim_fun open MA MI IstFull SpinLockName.release.
     winit_simF u_a 0.
+    (* process src precondition *)
     wsteps_l.
     iDestruct "ASM" as "[(% & TID & #LOCK & TKN & Q) %]".
     iDestruct "LOCK" as (? ?) "[% LOCK]".
     hss.
     wsteps_r.
+    (* tgt yield *)
     sch_yield_r. iFrame. clear nths; iIntros (nths0 st_s st_t) "IST TID".
-    iInv "LOCK" as "I" "Hcl".
-    SL_red.
+    (* open invariant *)
+    iInv "LOCK" as "I" "Hcl". SL_red.
     iDestruct "I" as "[LOCKED|UNLOCKED]".
-    { winline_r. wsteps_r. wforces_r. instantiate (1:= (_, _)).
+    { (* locked case *)
+      winline_r. wsteps_r. wforces_r. instantiate (1:= (_, _)).
       ss. instantiate (2:=(_, _)). ss.
       iSplitL "LOCKED"; iFrame; et.
       wsteps_r. iDestruct "GRT" as "[[POINTS_TO %] %]". hss.
       wsteps_r.
       iMod ("Hcl" with "[POINTS_TO Q TKN]") as "_". iRight. iFrame.
+      (* tgt yield *)
       sch_yield_r. iFrame. clear nths0; iIntros (nths st_s0 st_t0) "IST TID".
+      (* src yield *)
       sch_yield_l. wsteps_l. wforces_l. iFrame. iSplit; et. wstep. iFrame; et.
     }
-    { iDestruct "UNLOCKED" as "[POINTS_TO [Q' TKN']]".
+    { (* unlocked case - ex falso quodlibet *)
+      iDestruct "UNLOCKED" as "[POINTS_TO [Q' TKN']]".
       iCombine "TKN TKN'" gives %Hv. done.
     }
   (*FAST*)Admitted.
 
+  (* Construct HSim.t for summing up each simulation proofs *)
   Lemma sim : HSim.t open MA MI emp%I IstFull.
   Proof.
     init_sim.
@@ -141,7 +154,8 @@ End SpinLockIA.
 Section SpinLockIA.
   Context `{!invG α Σ Γ, !subG Γ Σ, !sinvG Σ Γ α β τ}.
   Context `{!SchAGΣ Σ, !SchAGΓ Γ, !memGΓ Γ, !SpinLockAGΓ Γ}.
-  Lemma wctxr (u : univ_id) (spc_s spc_user_s spc_mem : string → option fspec)
+  (* ctxr works as a unit in compositions of module simulations *)
+  Lemma ctxr (u : univ_id) (spc_s spc_user_s spc_mem : string → option fspec)
       (SchInSpc : spc_incl (SchAS.spc u spc_user_s) spc_s)
       (MemInSpc : spc_incl MemA.spc spc_s) :
     ctx_refines
